Add 4.8

ExampleProtocols.thy
@@ -7,7 +7,7 @@ begin
 (* Section 4: Example Protocols *)
 (* Section 4.1 *)
 
-(* Definition 4.1 *)
+(* Definition 4.1 Observed validators *)
 definition observed :: "state \<Rightarrow> validator set"
   where
     (* "observed s = {v. \<exists> m. v = sender m \<and> m \<in> s}" *)
@@ -18,12 +18,12 @@ fun later :: "(message * state) \<Rightarrow> state"
   where
     "later (m, s) = {m'. m' \<in> s \<and> m \<in> justification m'}"
 
-(* Definition 4.3 *)
+(* Definition 4.3 Messages From a Sender *)
 fun from_sender :: "(validator * state) \<Rightarrow> state"
   where
     "from_sender (v, s) = {m. m \<in> s \<and> sender m = v}"
 
-(* Definition 4.4 *)
+(* Definition 4.4 Message From a Group *)
 fun from_group :: "(validator set * state) \<Rightarrow> state"
   where
     "from_group (V, s) = {m. m \<in> s \<and> sender m \<in> V}"
@@ -33,9 +33,31 @@ fun later_from :: "(message * validator * state) \<Rightarrow> state"
   where
     "later_from (m, v, s) = later (m, s) \<inter> from_sender (v, s)"
 
-(* Definition 4.6 *)
+(* Definition 4.6 Latest Message *)
 definition latest_message :: "state \<Rightarrow> (validator \<Rightarrow> state)"
   where
     "latest_message s v = {m. m \<in> from_sender (v, s) \<and> later_from (m, v, s) = \<emptyset>}"
+
+(* Definition 4.7 Latest message driven estimator *)
+(* TODO *)
+
+(* Definition 4.8 Latest Estimates *)
+definition latest_estimates :: "state \<Rightarrow> validator \<Rightarrow> consensus_value set"
+  where
+    "latest_estimates s v = {est(m) | m. m \<in> latest_message s v}"
+
+(* Definition 4.9 Latest estimate driven estimator *)
+(* TODO *)
+
+(* Lemma 5 Non-equivocating validators have at most one latest message *)
+(* TODO *)
+
+(*
+lemma non_equivocating_validators_have_at_most_one_latest_message:
+  (* "\<forall> v \<in> V. v \<notin> equivocating_validators s \<Longrightarrow> count (latest_estimates s v) \<le> 1" *)
+  (* prove the contrapositive *)
+  "\<forall> v \<in> V. count (latest_estimates s v) > 1 \<Longrightarrow> v \<in> equivocating_validators s" 
+  apply (simp add: latest_estimates_def latest_message_def)
+*)
 
 end
